@prefix dct: <http://purl.org/dc/terms/> .
@prefix owl: <http://www.w3.org/2002/07/owl#> .
@prefix rdf: <http://www.w3.org/1999/02/22-rdf-syntax-ns#> .
@prefix xml: <http://www.w3.org/XML/1998/namespace> .
@prefix xsd: <http://www.w3.org/2001/XMLSchema#> .
@prefix foaf: <http://xmlns.com/foaf/0.1/> .
@prefix rdfs: <http://www.w3.org/2000/01/rdf-schema#> .
@prefix voaf: <http://purl.org/vocommons/voaf#> .
@prefix vann: <http://purl.org/vocab/vann/> .
@prefix vs: <http://www.w3.org/2003/06/sw-vocab-status/ns#> .
@prefix cc: <http://creativecommons.org/ns#> .
@prefix max: <http://maxime-lefrancois.info/me#> .

@base <https://w3id.org/function/ontology#> .
@prefix : <https://w3id.org/function/ontology#> .
<https://w3id.org/function/ontology>  rdf:type owl:Ontology ;

                                      rdf:type voaf:Vocabulary;
                                      
                                      vann:preferredNamespacePrefix "fno";
                                      
                                      vann:preferredNamespaceUri "https://w3id.org/function/ontology#";
                                      
                                      rdfs:label "the Function Ontology"@en ;
                                      
                                      dct:title "the Function Ontology"@en ;
                                      
                                      dct:description "The Function Ontology allows to declare and describe functions. The specification is online at http://users.ugent.be/~bjdmeest/function/"@en;
                                      
                                      rdfs:comment """-Version 0.4: added some properties
-Version 0.3: improved comments.
-Version 0.2: added extra metadata.
-Version 0.1: creation."""@en ;
                                      
                                      owl:versionIRI <https://w3id.org/function/ontology/0.4> ;
                                      owl:versionInfo "0.4" ;
                                      owl:priorVersion "https://w3id.org/function/ontology/0.3" ;
                                      
                                      rdfs:seeAlso <http://users.ugent.be/~bjdmeest/function/> ;
                                      
                                      dct:modified "2016-06-10"^^xsd:date ;
                                     
                                      dct:issued "2016-03-08"^^xsd:date ;
                                      
                                      owl:versionInfo "0.4"^^xsd:decimal ;
                                      
                                      dct:rights "Copyright © Ghent University – iMinds – Data Science Lab"@en ;
                                      
                                      cc:license <http://creativecommons.org/license/by/3.0/> ;
                                     
                                      foaf:primaryTopic <http://semweb.datasciencelab.be/ns/function> ;
                                      
                                      dct:creator [ 
                                      
                                      rdf:type foaf:Person ;
                                      
                                      foaf:mbox "mailto:Ben.DeMeester@UGent.be";
                                    
                                      foaf:name "Ben De Meester"@en
                                      
                                      ] ;
                                      
                                      dct:contributor [
                                      
                                      rdf:type foaf:Person ;
                                      
                                      foaf:mbox "mailto:Anastasia.dimou@UGent.be" ;
                                      
                                      foaf:name "Anastasia Dimou"@en
                                      
                                      ] ;
                                      dct:contributor max: .


#################################################################
#
#    Annotation properties
#
#################################################################


###  http://purl.org/dc/terms/issued

dct:issued rdf:type owl:AnnotationProperty .



###  http://purl.org/dc/terms/modified

dct:modified rdf:type owl:AnnotationProperty .



###  http://xmlns.com/foaf/0.1/primaryTopic

foaf:primaryTopic rdf:type owl:AnnotationProperty .





#################################################################
#
#    Datatypes
#
#################################################################


###  http://www.w3.org/2001/XMLSchema#date

xsd:date rdf:type rdfs:Datatype .





#################################################################
#
#    Object Properties
#
#################################################################


###  https://w3id.org/function/ontology#executes

:executes rdf:type owl:ObjectProperty ;
          
          rdfs:label "executes"@en ;
          
          rdfs:comment "Connects a function to an execution definition"@en ;
          
          rdfs:isDefinedBy <https://w3id.org/function/ontology#> ;
          
          vs:term_status "testing" ;
          
          rdfs:domain :Execution ;
          
          rdfs:range :Function .



###  https://w3id.org/function/ontology#expects

:expects rdf:type owl:ObjectProperty ;
         
         rdfs:label "expects"@en ;
         
         rdfs:comment "Connects a function description to an ordered list of zero or more parameter descriptions"@en ;
         
         rdfs:isDefinedBy <https://w3id.org/function/ontology#> ;
         
         vs:term_status "testing" ;
         
         rdfs:domain :Function ;
         
         rdfs:range rdf:List .



###  https://w3id.org/function/ontology#implements

:implements rdf:type owl:ObjectProperty ;
            
            rdfs:label "implements"@en ;
            
            rdfs:comment "Connects a function to an algorithm it implements. A function can implement 0..n algorithms."@en ;
            
            rdfs:isDefinedBy <https://w3id.org/function/ontology#> ;
            
            vs:term_status "testing" ;
            
            rdfs:range :Algorithm ;
            
            rdfs:domain :Function .



###  https://w3id.org/function/ontology#returns

:returns rdf:type owl:ObjectProperty ;
         
         rdfs:label "returns"@en ;
         
         rdfs:comment "Connects a description of a function to the description of the output"@en ;
         
         rdfs:isDefinedBy <https://w3id.org/function/ontology#> ;
         
         vs:term_status "testing" ;
         
         rdfs:domain :Function ;
         
         rdfs:range :Output .



###  https://w3id.org/function/ontology#solves

:solves rdf:type owl:ObjectProperty ;
        
        rdfs:label "solves"@en ;
        
        rdfs:comment "Connects a description of a function to the description of a problem it tries to solve."@en ;
        
        rdfs:isDefinedBy <https://w3id.org/function/ontology#> ;
        
        vs:term_status "testing" ;
        
        rdfs:domain :Function ;
        
        rdfs:range :Problem .



###  https://w3id.org/function/ontology#predicate

:predicate rdf:type rdf:Property ;
        
        rdfs:label "predicate"@en ;
        
        rdfs:comment "Connects a parameter description to the predicate used to link executions of this function to their parameter."@en ;
        
        rdfs:isDefinedBy <https://w3id.org/function/ontology#> ;
        
        vs:term_status "testing" ;
        
        rdfs:domain :Parameter ;
        
        rdfs:range rdf:Property .


###  https://w3id.org/function/ontology#type

:type rdf:type rdf:Property ;
        
        rdfs:label "type"@en ;
        
        rdfs:comment "Connects an output or a parameter description to the type of instances of these parameters or outputs."@en ;
        
        rdfs:isDefinedBy <https://w3id.org/function/ontology#> ;
        
        vs:term_status "testing" ;
        
        rdfs:range rdf:Property .




###  https://w3id.org/function/ontology#name

:name rdf:type rdf:Property ;
        
        rdfs:label "name"@en ;
        
        rdfs:comment "Connects an function or a parameter to its name."@en ;

        rdfs:subPropertyOf rdfs:label ;

        rdfs:range xsd:string ;
        
        rdfs:isDefinedBy <https://w3id.org/function/ontology#> ;
        
        vs:term_status "testing" ;

        rdfs:domain :Function .
        
###  https://w3id.org/function/ontology#required

:required rdf:type rdf:Property ;
        
        rdfs:label "required"@en ;
        
        rdfs:comment "Defines if a parameter or an output is required."@en ;

        rdfs:range xsd:boolean ;
        
        rdfs:isDefinedBy <https://w3id.org/function/ontology#> ;
        
        vs:term_status "testing" .

###  https://w3id.org/function/ontology#nullable

:nullable rdf:type rdf:Property ;
        
        rdfs:label "nullable"@en ;
        
        rdfs:comment "Defines if a parameteris nullable."@en ;

        rdfs:range xsd:boolean ;
        
        rdfs:isDefinedBy <https://w3id.org/function/ontology#> ;
        
        vs:term_status "testing" .




#################################################################
#
#    Classes
#
#################################################################


###  https://w3id.org/function/ontology#Algorithm

:Algorithm rdf:type owl:Class ;
           
           rdfs:label "Algorithm"@en ;
           
           rdfs:comment "A declaration of an algorithm. An algorithm is a specified set of instructions, independent of its implementation. There is no one-to-one mapping between an algorithm and a problem."@en ;
           
           vs:term_status "testing" ;
           
           rdfs:isDefinedBy <https://w3id.org/function/ontology#> .



###  https://w3id.org/function/ontology#Execution

:Execution rdf:type owl:Class ;
           
           rdfs:label "Execution"@en ;
           
           rdfs:comment "An execution is the connection between a function and its input and output values."@en ;
           
           vs:term_status "testing" ;
           
           rdfs:isDefinedBy <https://w3id.org/function/ontology#> .



###  https://w3id.org/function/ontology#Function

:Function rdf:type owl:Class ;
          
          rdfs:label "Function"@en ;
          
          rdfs:comment "The declared function"@en ;
          
          vs:term_status "testing" ;
          
          rdfs:isDefinedBy <https://w3id.org/function/ontology#> .



###  https://w3id.org/function/ontology#Output

:Output rdf:type owl:Class ;
        
        rdfs:label "Output"@en ;
        
        rdfs:comment "The definition of an output of a function"@en ;
        
        vs:term_status "testing" ;
        
        rdfs:isDefinedBy <https://w3id.org/function/ontology#> .



###  https://w3id.org/function/ontology#Parameter

:Parameter rdf:type owl:Class ;
           
           rdfs:label "Parameter"@en ;
           
           rdfs:comment "The definition of a parameter to a certain function"@en ;
           
           vs:term_status "testing" ;
           
           rdfs:isDefinedBy <https://w3id.org/function/ontology#> .



###  https://w3id.org/function/ontology#Problem

:Problem rdf:type owl:Class ;
         
         rdfs:label "Problem"@en ;
         
         rdfs:comment "A certain problem that a function solves"@en ;
         
         vs:term_status "testing" ;
         
         rdfs:isDefinedBy <https://w3id.org/function/ontology#> .



###  http://xmlns.com/foaf/0.1/Document

foaf:Document rdf:type owl:Class .
                                     
                                     
